\subsection{ARC: Zenithal equidistant}

  The Zenithal equidistant projection is the simple case in which:
  \begin{equation}
    R = \rho
  \end{equation}

  \subsubsection{Projection}

    From Eq. (\ref{eq:zenithal.X}), (\ref{eq:zenithal.Y}), (\ref{eq:zen.x}) and (\ref{eq:zen.y}),
    we simply have:
    \begin{eqnarray}
      X & = & \rho\cos\theta = \frac{\rho}{\sin\rho}y
              = \frac{\arcsin\sqrt{y^2 + z^2}}{\sqrt{y^2 + z^2}}y
              = y\arcsinc r \\
      Y & = & \rho\sin\theta = \frac{\rho}{\sin\rho}z
              = \frac{\arcsin\sqrt{y^2 + z^2}}{\sqrt{y^2 + z^2}}z
              = z\arcsinc r 
    \end{eqnarray}
    In practice for large angular distances (let us say $\rho>\pi/2$), we 
    replace $\arcsinc r$ by $\arccos(x) / r$ for a better numercial precision.

  \subsubsection{Deprojection}
  
    We easily inverse the previous equations:
    \begin{equation}
      X^2 + Y^2 = \rho^2.
    \end{equation}
    Using Eq. (\ref{eq:zen.x}), we deduce $x$
    \begin{equation}
      x = \cos\rho = \cos(\sqrt{X^2 + Y^2})
    \end{equation}
    and from Eq. (\ref{eq:zen.y}), (\ref{eq:zen.z}), (\ref{eq:zenithal.X}) and (\ref{eq:zenithal.Y})
    we deduce
    \begin{eqnarray}
      y & = & X \frac{\sin\rho}{\rho} = X \sinc(\sqrt{X^2 + Y^2}) \\  
      z & = & Y \frac{\sin\rho}{\rho} = Y \sinc(\sqrt{X^2 + Y^2})
    \end{eqnarray}

