\subsection{ZEA: Zenithal equal-area}

  The zenithal equal-area projection is the quite simple case in which
  \begin{equation}
    R = 2\sin\frac{\rho}{2}.
  \end{equation}

 \subsubsection{Projection}

  We develop the expression of the Euclidean distance $R$
  using Eq. (\ref{eq:cos2x}) and then Eq. (\ref{eq:zen.x}):
  \begin{eqnarray}
    R^2 & = & 4\sin^2\frac{\rho}{2} \\
        & = & 4\frac{1 - \cos\rho}{2} \\
        & = & 2(1 - x)
  \end{eqnarray}
  So the projection formulae are
  \begin{eqnarray}
    X & = & \sqrt{2(1 - x)} \frac{y}{\sin\rho} \\
      & = & \sqrt{\frac{2(1 - x)}{1 - x^2}} y \\
      & = & \sqrt{\frac{2}{1+x}}y \label{eq:zea.proj.X}\\
    Y & = & \sqrt{2(1 - x)} \frac{z}{\sin\rho} \\
      & = & \sqrt{\frac{2}{1+x}}z \label{eq:zea.proj.Y}
  \end{eqnarray}

  \subsubsection{Deprojection}

    We find the expression of $x$ from $R^2=X^2+Y^2$:
    \begin{eqnarray}
      R^2 & = & \frac{2}{1+x}r \\
          & = & \frac{2}{1+x}(1-x^2) \\
          & = & \frac{2}{1+x}(1+x)(1-x) \\
          & = & 2(1-x)
    \end{eqnarray}
    So
    \begin{equation}
      x = 1 - \frac{R^2}{2} = 1 - \frac{X^2+Y^2}{2}
    \end{equation}
    We now reinject this expression of $x$ in the projection formulae Eq. (\ref{eq:zea.proj.X}) and (\ref{eq:zea.proj.Y})
    To obtain 
    \begin{eqnarray}
      y & = & \sqrt{1-\frac{R^2}{4}}X = \sqrt{1-\frac{X^2+Y^2}{4}}X \\
      z & = & \sqrt{1-\frac{R^2}{4}}Y = \sqrt{1-\frac{X^2+Y^2}{4}}Y
    \end{eqnarray}
 

