\section{Trigonometry formulary}

  \subsection{Fundamental relations}

    \begin{eqnarray}
      \cos^2a + \sin^2x & = & 1 \label{eq:cos2sin2eq1} \\
      \frac{1}{\cos^2}  & = & 1 + \tan^2 x \label{eq:1ocxeq1ptx}
    \end{eqnarray}

  \subsection{Addition formulae}

  \begin{eqnarray}
    \cos(a + b) & = & \cos a \cos b - \sin a \sin b \label{eq:cosapb} \\
    \cos(a - b) & = & \cos a \cos b + \sin a \sin b \label{eq:cosamb} \\
    \sin(a + b) & = & \sin a \cos b + \cos a \sin b \label{eq:sinapb} \\
    \sin(a - b) & = & \sin a \cos b - \cos a \sin b \label{eq:sinamb}
  \end{eqnarray}

  \subsection{Double angle formulae}

  We deduce from the above equations (and Eq. \ref{eq:1ocxeq1ptx}) that:
  \begin{eqnarray}
    \cos(2x) & = & \cos^2 x - \sin^2 x = 2\cos^2 x - 1 = 1 - 2\sin^2 x \label{eq:cos2x} \\
    \sin(2x) & = & 2\sin x \cos x \label{eq:sin2x} \\
    \tan(2x) & = & \frac{2\tan x}{1 + \tan^2x} \label{eq:tan2x}
  \end{eqnarray}

  \subsection{Semi-angle formulae}

    \begin{eqnarray}
      \cos^2 x & = & \frac{1 + \cos(2x)}{2} \label{eq:cosx2} \\
      \sin^2 x & = & \frac{1 - \cos(2x)}{2} \label{eq:sinx2} \\
      \tan^2 x & = & \frac{\sin(2x)}{1 + \cos(2x)} = \frac{1 - \cos(2x)}{\sin(2x)} \label{eq:tanx2}
    \end{eqnarray}


  \subsection{Trigonometric functions depending on inverse trigonometric functions}  

  \begin{eqnarray}
      \cos(\arccos x) &= & x                        \label{eq:cosarccos} \\
      \cos(\arcsin x) &= & \sqrt{1 - x^2}           \label{eq:cosarcsin} \\
      \cos(\arctan x) &= & \frac{1}{\sqrt{1 + x^2}} \label{eq:cosarctan} \\
      \sin(\arccos x) &= & \sqrt{1 - x^2}           \label{eq:sinarccos} \\
      \sin(\arcsin x) &= &  x                       \label{eq:sinarcsin} \\
      \sin(\arctan x) &= & \frac{x}{\sqrt{1 + x^2}} \label{eq:sinarctan} \\
      \tan(\arccos x) &= & \frac{\sqrt{1 - x^2}}{x} \label{eq:tanarccos} \\
      \tan(\arcsin x) &= & \frac{x}{\sqrt{1 - x^2}} \label{eq:tanarcsin} \\
      \tan(\arctan x) &= & x                        \label{eq:tanarctan}
  \end{eqnarray} 

  %\begin{equation}
  %  \begin{array}{r@=l r@=l r@=l}
  %    \cos(\arccos x) & x 
  %    & \cos(\arcsin x) & \sqrt{1 - x^2}
  %    & \cos(\arctan x) & \frac{1}{\sqrt{1 + x^2}} \\
  %    \sin(\arccos x) & \sqrt{1 - x^2}
  %    & \sin(\arcsin x) &  x
  %    & \sin(\arctan x) & \frac{x}{\sqrt{1 + x^2}} \\
  %    \tan(\arccos x) & \frac{\sqrt{1 - x^2}}{x}
  %    & \tan(\arcsin x) & \frac{x}{\sqrt{1 - x^2}}
  %    & \tan(\arctan x) & x
  %  \end{array}
  %\end{equation}

